Trying to add simple products (wip)

formalization/config.v
@@ -6,5 +6,9 @@ Class Reflection := {
   reflectionFlag : Type
 }.
 
+Class SimpleProducts := {
+  simpleproductsFlag : Type
+}.
+
 Inductive Yes : Type := yes.
 Inductive No : Type := .
