formalization/negfunext.v
@@ -1,0 +1,54 @@
+(* In order to test our formalisation, we propose our own formalisation of a
+   model that negates function extensionality, following Simon Boulier,
+   Pierre-Marie Pédrot et Nicolas Tabareau.
+*)
+
+Require config.
+Require Import config_tactics.
+
+Require Import syntax.
+Require Import tt.
+
+(* Source type theory *)
+Module Stt.
+
+  Section Stt.
+
+  Local Instance hasPrecond : config.Precond
+    := {| config.precondFlag := config.Yes |}.
+  Context `{configReflection : config.Reflection}.
+
+  Definition isctx := isctx.
+  Definition issubst := issubst.
+  Definition istype := istype.
+  Definition isterm := isterm.
+  Definition eqctx := eqctx.
+  Definition eqsubst := eqsubst.
+  Definition eqtype := eqtype.
+  Definition eqterm := eqterm.
+
+  End Stt.
+
+End Stt.
+
+(* Target type theory *)
+Module Ttt.
+
+  Section Ttt.
+
+  Local Instance hasPrecond : config.Precond
+    := {| config.precondFlag := config.No |}.
+  Context `{configReflection : config.Reflection}.
+
+  Definition isctx := isctx.
+  Definition issubst := issubst.
+  Definition istype := istype.
+  Definition isterm := isterm.
+  Definition eqctx := eqctx.
+  Definition eqsubst := eqsubst.
+  Definition eqtype := eqtype.
+  Definition eqterm := eqterm.
+
+  End Ttt.
+
+End Ttt.
