formalization/ptt_inversion.v
@@ -10,6 +10,7 @@ Section PttInversion.
 
 Local Instance hasPrecond : config.Precond := {| config.precondFlag := config.Yes |}.
 Context `{ConfigReflection : config.Reflection}.
+Context `{configSimpleProducts : config.SimpleProducts}.
 
 Definition CtxExtendInversion G A (H : isctx (ctxextend G A)) :
   isctx G * istype G A.
@@ -25,12 +26,12 @@ Proof.
   - { split ; [(split ; [split | idtac]) | idtac].
 
       - assumption.
-      - apply (@TyCtxConv _ _ G0 G) ; auto.
+      - apply (@TyCtxConv _ _ _ G0 G) ; auto.
         now apply TyIdInversion with (u := u) (v := v).
-      - apply (@TermCtxConv _ _ G0 G) ; auto.
+      - apply (@TermCtxConv _ _ _ G0 G) ; auto.
         + now apply TyIdInversion with (u := u) (v:= v).
         + now config apply TyIdInversion with (u := u) (v:= v).
-      - apply (@TermCtxConv _ _ G0 G) ; auto.
+      - apply (@TermCtxConv _ _ _ G0 G) ; auto.
         + now apply TyIdInversion with (u := u) (v:= v).
         + now config apply TyIdInversion with (u := u) (v:= v).
     }
@@ -51,9 +52,9 @@ Proof.
 
   - { split ; [ split | idtac ].
       - assumption.
-      - apply (@TyCtxConv _ _ G0 G) ; auto.
+      - apply (@TyCtxConv _ _ _ G0 G) ; auto.
         now apply (TyProdInversion G0 A B).
-      - apply (@TyCtxConv _ _ (ctxextend G0 A) (ctxextend G A)).
+      - apply (@TyCtxConv _ _ _ (ctxextend G0 A) (ctxextend G A)).
         + now apply (TyProdInversion G0 A B).
         + apply EqCtxExtend ; auto.
           * now capply (TyProdInversion G0 A B).
@@ -64,7 +65,7 @@ Proof.
           now apply (TyProdInversion G0 A B).
         + capply CtxExtend.
           * assumption.
-          * apply (@TyCtxConv _ _ G0 G) ; auto.
+          * apply (@TyCtxConv _ _ _ G0 G) ; auto.
             now apply (TyProdInversion G0 A B).
     }
 
